minor update

systemt/intensional/partial_completeness.v
@@ -7,88 +7,83 @@ Definition SemTyp := D -> Prop.
 
 Definition SemEnv := Env -> Prop.
 
-Definition Top : SemTyp := 
- fun d => forall n, exists v, Rⁿᶠ ⦇ n ⦈ d ↘ v.
+Definition SemTypTop : SemTyp := 
+  fun d => forall n, exists v, Rⁿᶠ ⦇ n ⦈ d ↘ v.
 
-Notation "d ∈ ⊤" := (Top d)
-   (at level 55, no associativity).
+Notation "d ∈ ⊤" := (SemTypTop d)
+  (at level 55, no associativity).
 
-Definition Bot : Dne -> Prop :=
+Definition SemTypBot : Dne -> Prop :=
  fun e => forall n, exists u, Rⁿᵉ ⦇ n ⦈ e ↘ u.
 
-Notation "e ∈ ⊥" := (Bot e)
-   (at level 55, no associativity).
+Notation "e ∈ ⊥" := (SemTypBot e)
+  (at level 55, no associativity).
 
 Reserved Notation "d ∈ '𝒩' "
   (at level 55, no associativity).
-Inductive SemNat : SemTyp :=
- | snat_zero : d_zero ∈ 𝒩
- | snat_suc : forall d,
+Inductive SemTypNat : SemTyp :=
+ | st_nat_zero : d_zero ∈ 𝒩
+ | st_nat_suc : forall d,
     d ∈ 𝒩 ->
     d_suc d ∈ 𝒩
- | snat_bot : forall e,
+ | st_nat_bot : forall e,
     e ∈ ⊥ ->
-    SemNat (d_ne e)
-where " d ∈ '𝒩' " := (SemNat d).
+    SemTypNat (d_ne e)
+where " d ∈ '𝒩' " := (SemTypNat d).
 
-Definition SemArr : SemTyp -> SemTyp -> SemTyp :=
-   fun A B f => forall a, A a -> exists b, B b /\ f ∙ a ↘ b.
+Definition SemTypArr : SemTyp -> SemTyp -> SemTyp :=
+  fun A B f => forall a, A a -> exists b, B b /\ f ∙ a ↘ b.
 
 Fixpoint interp_typ (T : Typ) : SemTyp :=
-   match T with 
-   | typ_nat => SemNat 
-   | typ_arr S' T' => SemArr (interp_typ S') (interp_typ T')
-   end.
+  match T with 
+  | typ_nat => SemTypNat 
+  | typ_arr S' T' => SemTypArr (interp_typ S') (interp_typ T')
+  end.
 
 Notation "⟦ T ⟧T" := (interp_typ T)
-   (at level 55, no associativity).
-
-(* Scheme d_ind := Induction for D Sort Prop
-  with dne_ind := Induction for Dne Sort Prop.
-
-Combined Scheme d_dne_mutind from d_ind, dne_ind. *)
+  (at level 55, no associativity).
 
 Lemma bot_subset_T_subset_top : forall T,
-   (forall e, e ∈ ⊥ -> ⟦ T ⟧T (d_ne e)) /\
-   (forall d, ⟦ T ⟧T d -> d ∈ ⊤).
-Proof with eauto using SemNat, RNeRel, RNfRel.
-   intros. induction T; split; try simpl...
-   - intros. dependent induction H.
-     + unfold Top. intros...
-     + unfold Top in *.
-       intros. specialize (IHSemNat n).
-       destruct IHSemNat as [v]...
-     + unfold Top in *. unfold Bot in *.
-       intros. specialize (H n).
-       destruct H as [u]...
-   - intros.
-     unfold Bot in *. 
-     unfold SemArr. intros.
-     exists (d_ne (dn_app e a)). split.
-     + destruct IHT1. 
-       destruct IHT2.
-       apply H3. intros.
-       apply H2 in H0. unfold Top in H0.
-       specialize (H n).
-       specialize (H0 n).
-       destruct H as [u]. destruct H0 as [v]...
-     + econstructor.
-   - intros. unfold SemArr in *.
-     unfold Top in *. intros. 
-     destruct IHT1.
-     destruct IHT2.
-     specialize (H (d_ne (dn_l n))).
-     assert ((⟦ T1 ⟧T) (d_ne (dn_l n))). {
-       eapply H0. unfold Bot. intros...
-     }
-     apply H in H4. destruct H4 as [b]. destruct H4 as [Hb Happ].
-     dependent destruction Happ.
-     + eapply H3 with (n:=S n) in Hb. 
-       destruct Hb as [v]. exists (nf_abs v). 
-       eapply rnf_abs; eauto.
-     + eapply H3 with (n:=n) in Hb.
-       destruct Hb as [v]. dependent destruction H4.
-       dependent destruction H4...
+  ( forall e, e ∈ ⊥ -> ⟦ T ⟧T (d_ne e) ) /\
+  ( forall d, ⟦ T ⟧T d -> d ∈ ⊤ ).
+Proof with eauto using SemTypNat, RNeRel, RNfRel.
+  intros. induction T; split; try simpl...
+  - intros. dependent induction H.
+    + unfold SemTypTop. intros...
+    + unfold SemTypTop in *.
+      intros. specialize (IHSemTypNat n).
+      destruct IHSemTypNat as [v]...
+    + unfold SemTypTop in *. unfold SemTypBot in *.
+      intros. specialize (H n).
+      destruct H as [u]...
+  - intros.
+    unfold SemTypBot in *. 
+    unfold SemTypArr. intros.
+    exists (d_ne (dn_app e a)). split.
+    + destruct IHT1. 
+      destruct IHT2.
+      apply H3. intros.
+      apply H2 in H0. unfold SemTypTop in H0.
+      specialize (H n).
+      specialize (H0 n).
+      destruct H as [u]. destruct H0 as [v]...
+    + econstructor.
+  - intros. unfold SemTypArr in *.
+    unfold SemTypTop in *. intros. 
+    destruct IHT1.
+    destruct IHT2.
+    specialize (H (d_ne (dn_l n))).
+    assert ((⟦ T1 ⟧T) (d_ne (dn_l n))). {
+      eapply H0. unfold SemTypBot. intros...
+    }
+    apply H in H4. destruct H4 as [b]. destruct H4 as [Hb Happ].
+    dependent destruction Happ.
+    + eapply H3 with (n:=S n) in Hb. 
+      destruct Hb as [v]. exists (nf_abs v). 
+      eapply rnf_abs; eauto.
+    + eapply H3 with (n:=n) in Hb.
+      destruct Hb as [v]. dependent destruction H4.
+      dependent destruction H4...
 Qed.
 
 Corollary bot_subset_T : forall e T, 
@@ -99,7 +94,8 @@ Proof.
 Qed.
 
 Corollary T_subset_top : forall d T, 
-  ⟦ T ⟧T d -> d ∈ ⊤.
+  ⟦ T ⟧T d -> 
+  d ∈ ⊤.
 Proof.
   specialize bot_subset_T_subset_top. intros. specialize (H T). intuition. 
 Qed.
